examples/loops_proofs.v
@@ -45,3 +45,39 @@ Proof.
     rewrite e_if, bvAdd_id_r.
     reflexivity.
 Qed.
+
+
+(* Add `add_loop_spec_ref` to the hint database. Unfortunately, Coq will not unfold refinesFun
+   and add_loop_spec when rewriting, and the only workaround I know right now is this :/ *)
+Definition add_loop_spec_ref' : ltac:(let tp := type of add_loop_spec_ref in
+                                      let tp' := eval unfold refinesFun, add_loop_spec in tp
+                                       in exact tp') := add_loop_spec_ref.
+Hint Rewrite add_loop_spec_ref' : refinesM.
+
+Lemma no_errors_compare : refinesFun compare (fun _ _ => noErrorsSpec).
+Proof.
+  unfold compare, compare__tuple_fun, noErrorsSpec.
+  time "no_errors_add_loop" prove_refinement.
+Qed.
+
+Definition compare_spec (x y : {_ : bitvector 64 & unit}) : CompM {_ : bitvector 64 & unit} :=
+  orM (     assertM (isBvslt _ (intToBv _ 0) (bvAdd _ (projT1 x) (projT1 y)))
+                    >> returnM (existT _ (intToBv _ 1) tt))
+      (orM (assertM (isBvslt _ (bvAdd _ (projT1 x) (projT1 y)) (intToBv _ 0))
+                    >> returnM (existT _ (intToBv _ (-1)) tt))
+           (assertM (bvAdd _ (projT1 x) (projT1 y) = intToBv _ 0)
+                    >> returnM (existT _ (intToBv _ 0) tt))).
+
+Lemma compare_spec_ref : refinesFun compare compare_spec.
+Proof.
+  unfold compare, compare__tuple_fun, compare_spec.
+  time "no_errors_add_loop" prove_refinement.
+  - continue_prove_refinement_left.
+    assumption.
+  - continue_prove_refinement_right;
+    continue_prove_refinement_left.
+    assumption.
+  - continue_prove_refinement_right;
+    continue_prove_refinement_right.
+    apply isBvsle_antisymm; assumption.
+Qed.
